TROUBLESHOOTING.md
@@ -1,6 +1,8 @@
 # On `induction` rule
 
-Sometimes the induction hypothesis needs to be univerally quantified on a
+## RULE: Think about universally quantifying certain variables in induction hypothesis
+
+Sometimes the induction hypothesis needs to be universally quantified on a
 particular variable. When this happens use `arbitrary`.
 
     apply (induction x arbitrary: y)
@@ -9,3 +11,24 @@ particular variable. When this happens use `arbitrary`.
 
 See p20 - p21 of book for more details. Also see the
 *Wed 27 Sep 2017* entry in [LOG.md](LOG.md)
+
+# On simplification rules
+
+## RULE: In equality lemmas order can matter
+
+In lemmas of the form "a = b" the _order can matter_. Try reversing the
+order and see if that help your proofs.
+
+# Intermediate lemmas
+
+## RULE: If proving something about a function that relies on helper functions, prove intermediate lemmas on the helper functions
+
+Example. In Exercise 3.9 I needed to prove
+
+    pbval (dnf_of_nnf b) s = pbval b s
+
+`dnf_of_nnf` used a helper function `dist` so it was necessary to prove:
+
+    pbval (dist a b) s = pbval (AND a b) s
+
+Looking at the goals carefully let me realise this.
